bin/commands/cgen.ml
@@ -23,15 +23,57 @@ let list_gen_correct : int list t =
   in
   aux len
 
+let rec bst_gen (low : int) (high : int) : int Tree.t t =
+ fun r ->
+  if high <= low + 1 then Tree.Leaf
+  else
+    Gen.frequencyl
+      [
+        (* (1, Tree.Leaf); *)
+        ( 1,
+          let x = Gen.int_range (low + 1) (high - 1) r in
+          let lt = (bst_gen low x) r in
+          let rt = (bst_gen x high) r in
+          Tree.Node (x, lt, rt) );
+      ]
+      r
+
+let rec is_bst (low : int) (high : int) = function
+  | Tree.Leaf -> true
+  | Tree.Node (x, lt, rt) ->
+      if low < x && x < high then is_bst low x lt && is_bst x high rt else false
+
+let sized_gen (low : int) (high : int) : int Tree.t t =
+  Gen.(
+    sized_size (int_range 0 (high - low))
+    @@ fix (fun self n ->
+           match n with
+           | 0 -> pure Tree.Leaf
+           | n ->
+               frequency
+                 [
+                   (1, pure Tree.Leaf);
+                   ( 2,
+                     map3
+                       (fun x lt rt -> Tree.Node (x, lt, rt))
+                       (int_range low high)
+                       (self (n - 1))
+                       (self (n - 1)) );
+                 ]))
+
 let test (num : int) =
-  let ls1 = Gen.generate ~n:num list_gen_wrong in
-  let () = Printf.printf "list_gen_wrong:\n" in
+  let ls1 = Gen.generate ~n:num (bst_gen 0 4) in
+  let ls1 = List.filter (is_bst 0 4) ls1 in
+  let ls1 = List.slow_rm_dup (Tree.eq ( = )) ls1 in
   let () =
-    List.iter (fun l -> Printf.printf "[%s]\n" (IntList.to_string l)) ls1
+    List.iter (fun t -> Printf.printf "%s\n" @@ Tree.layout string_of_int t) ls1
   in
-  let () = Printf.printf "\nlist_gen_correct:\n" in
-  let ls2 = Gen.generate ~n:num list_gen_correct in
+  let () = Printf.printf "bst: %i\n" @@ List.length ls1 in
+  let ls1 = Gen.generate ~n:(num * 1000) (sized_gen 0 4) in
+  let ls1 = List.filter (is_bst 0 4) ls1 in
+  let ls1 = List.slow_rm_dup (Tree.eq ( = )) ls1 in
   let () =
-    List.iter (fun l -> Printf.printf "[%s]\n" (IntList.to_string l)) ls2
+    List.iter (fun t -> Printf.printf "%s\n" @@ Tree.layout string_of_int t) ls1
   in
+  let () = Printf.printf "bst: %i\n" @@ List.length ls1 in
   ()
