data/benchmark/elrond/bankersq/prog.ml
@@ -1,0 +1,5 @@
+let bankersq_gen (lenf : int) : int bankersq =
+  let (lenr : int) = int_range 0 lenf in
+  let (f : int stream) = stream_gen lenf in
+  let (r : int stream) = stream_gen lenr in
+  Bankersq (lenf, f, lenr, r)
