data/benchmark/elrond/leftisthp/_under.ml
@@ -1,0 +1,16 @@
+let[@library] int_range =
+  let (x : [%over: int]) = (true : [%v: int]) in
+  let (y : [%over: int]) = (true : [%v: int]) in
+  (x <= v && v <= y : [%v: int])
+
+let[@library] int_gen =
+  let (dummy : [%over: unit]) = (true : [%v: unit]) in
+  (true : [%v: int])
+
+let[@library] bool_gen =
+  let (dummy : [%over: unit]) = (true : [%v: unit]) in
+  (true : [%v: bool])
+
+let leftisthp_gen =
+  let (s : [%over: int]) = (0 <= v : [%v: int]) in
+  (len v s : [%v: int leftisthp])
