data/benchmark/elrond/leftisthp/prog.ml
@@ -1,0 +1,10 @@
+let rec leftisthp_gen (size : int) : int leftisthp =
+  let (b : bool) = size == 0 in
+  if b then Lhpleaf
+  else
+    let (size1 : int) = size - 1 in
+    let (lt : int leftisthp) = leftisthp_gen size1 in
+    let (size2 : int) = int_range 0 size1 in
+    let (rt : int leftisthp) = leftisthp_gen size2 in
+    let (n : int) = int_gen () in
+    Lhpnode (n, lt, rt, size2)
