data/typedecs.ml
@@ -1,8 +1,4 @@
 (* The datatype constructor should use the lower case instead of the first char *)
-type 'a leftisthp =
-  | Lhpleaf
-  | Lhpnode of int * 'a * 'a leftisthp * 'a leftisthp
-
 type 'a pairinghp = Phpleaf | Phpnode of 'a * 'a pairinghp list
 type 'a tree = Leaf | Node of 'a * 'a tree * 'a tree
 type 'a heap = Hempty | Hnode of 'a * 'a heap * 'a heap
@@ -11,5 +7,12 @@ type 'a binomialhp = Bhpleaf | Bhpnode of int * 'a * 'a binomialhp list
 type 'a rbtree = Rbtleaf | Rbtnode of bool * 'a rbtree * 'a * 'a rbtree
 type 'a skewhp = Shpnode of int * 'a * 'a list * 'a skewhp list
 type 'a splayhp = Sphpleaf | Sphpnode of 'a splayhp * 'a * 'a splayhp
-type 'a unbset = Usleaf | Usnode of 'a unbset * 'a * 'a unbset
+type 'a unbset = Usleaf | Usnode of 'a * 'a unbset * 'a unbset
 type 'a batchedq = Batchedq of 'a list * 'a list
+type 'a lazyty = Lazyty of 'a
+type 'a stream = Streamnil | Streamlazycons of 'a * 'a stream lazyty
+type 'a bankersq = Bankersq of int * 'a stream * int * 'a stream
+
+type 'a leftisthp =
+  | Lhpleaf
+  | Lhpnode of 'a * 'a leftisthp * 'a leftisthp * int
