proof/LinearContext.v
@@ -5,19 +5,43 @@ Import ListNotations.
 
 Definition linear_context (A : Type) := list (string * A).
 
-Definition empty {A:Type} : linear_context A := [].
+Definition l_empty {A:Type} : linear_context A := nil.
 
-Definition find {A:Type} (ctx: linear_context A) (name: string) : option A.
+(* Implemenetd as find the right most one *)
+
+Fixpoint l_find_right_most {A:Type} (ctx: linear_context A) (name: string) :=
+  match ctx with
+  | [] => None
+  | (x, xty)::ctx =>
+      match l_find_right_most ctx name with
+      | None => if String.eqb x name then Some xty else None
+      | Some xty => Some xty
+      end
+  end.
+
+Lemma l_find_right_most_some_spec {A:Type}: forall (ctx: linear_context A) (name: string) (tau: A),
+  l_find_right_most ctx name = Some tau ->
+  (exists ctx1 ctx2,
+      ctx = ctx1 ++ ((name, tau)::nil) ++ ctx2 /\
+        l_find_right_most ctx2 name = None
+  ).
 Admitted.
 
-Definition update {A : Type} (m : linear_context A) (x : string) (v : A) : linear_context A.
-Admitted.
+(* update the to left most *)
+Definition l_append {A : Type} (m : linear_context A) (x : string) (v : A) : linear_context A := m ++ [(x, v)].
 
-Definition rev_ctx {A : Type} (m : linear_context A): linear_context A.
-Admitted.
+(* Not same name *)
+Definition linear_context_inv {A:Type} (ctx: linear_context A) := True.
 
-Notation "x '|-c>' v ';' m" := (update m x v)
-                                (at level 100, v at next level, right associativity).
-Notation "x '|-c>' v" := (update empty x v)
-                          (at level 100).
+Notation " m '<l>' x ':l:' ty " := (l_append m x ty) (at level 80).
 
+Global Hint Rewrite app_nil_l: core.
+Global Hint Rewrite app_nil_r: core.
+
+(* Declare Scope linear_context_scope. *)
+(* Notation "G[ ]" := nil (format "G[ ]") : linear_context_scope. *)
+(* Notation " context 'G::' x " := (cons x context) (at level 80) : linear_context_scope. *)
+(* Notation "G[ x ]" := (cons x nil) : linear_context_scope. *)
+(* Notation "G[ x ; y ]" := (cons y (cons x nil)) : linear_context_scope. *)
+(* Notation "G[ x ; y ; z ]" := (cons z (cons y (cons x nil))) : linear_context_scope. *)
+(* Notation "G[ x ; y ; z ; a ]" := (cons a (cons z (cons y (cons x nil)))) : linear_context_scope. *)
