proof/CoreLangSimp.v
@@ -1,0 +1,132 @@
+(** * MoreStlc: More on the Simply Typed Lambda-Calculus *)
+
+Set Warnings "-notation-overridden,-parsing".
+From PLF Require Import Maps.
+From PLF Require Import Types.
+From PLF Require Import Smallstep.
+
+Ltac invert :=
+  match goal with | H : ?T |- _ =>
+                      match type of T with Prop => solve [exfalso; apply H; auto]
+                      end
+  end.
+
+(* ----------------------------------------------------------------- *)
+(** *** Syntax *)
+
+Inductive basic_ty : Type :=
+| TNat   : basic_ty
+| TBool  : basic_ty.
+
+Inductive constant : Type :=
+| cbool: bool -> constant
+| cnat : nat -> constant.
+
+Lemma constant_eqb_spec: forall (c c': constant), c = c' \/ c <> c'.
+Admitted.
+
+Inductive ty : Type :=
+| TBasic : basic_ty -> ty
+| TArrow : ty -> ty -> ty.
+
+Coercion TBasic : basic_ty >-> ty.
+Coercion cbool : bool >-> constant.
+Coercion cnat : nat >-> constant.
+Notation " t1 't-->' t2 " := (TArrow t1 t2) (at level 20).
+
+Inductive biop : Type :=
+| op_plus
+| op_eq
+| op_lt.
+
+Inductive value : Type :=
+| vconst : constant -> value
+| vvar : string -> value
+| vlam : string -> ty -> tm -> value
+with tm : Type :=
+| texn
+| tvalue: value -> tm
+| tlete: string -> tm -> tm -> tm
+| tletbiop: string -> biop -> value -> value -> tm -> tm
+| tletapp: string -> value -> value -> tm -> tm.
+
+Scheme value_mutual_rec := Induction for value Sort Type
+    with tm_mutual_rec := Induction for tm Sort Type.
+
+Coercion vconst : constant >-> value.
+Coercion vvar : string >-> value.
+Coercion tvalue : value >-> tm.
+
+Definition is_value (e: tm) :=
+  match e with
+  | tvalue _ => true
+  | _ => false
+  end.
+
+Lemma is_value_value_exists: forall e, is_value e = true -> exists v, e = tvalue v.
+Proof.
+  intros.
+  destruct e; inversion H; subst. exists v. auto.
+Qed.
+
+Fixpoint subst (x:string) (s:value) (t:tm) : tm :=
+  match t with
+  |  texn => t
+  | tvalue v => tvalue (value_subst x s v)
+  | tlete x' t1 t2 =>
+      tlete x' (subst x s t1) (if String.eqb x x' then t2 else (subst x s t2))
+  | tletbiop x' op v1 v2 t2 =>
+      tletbiop x' op (value_subst x s v1) (value_subst x s v2) (if String.eqb x x' then t2 else (subst x s t2))
+  | tletapp x' v1 v2 t2 =>
+      tletapp x' (value_subst x s v1) (value_subst x s v2)
+              (if String.eqb x x' then t2 else (subst x s t2))
+  end
+with value_subst (x:string) (s:value) (t:value) : value :=
+       match t with
+       |  vconst _ => t
+       |  vvar y => if String.eqb x y then s else t
+       |  vlam y T t1 => vlam y T (if String.eqb x y then t1 else (subst x s t1))
+       end.
+
+Definition apply_op (op: biop) (a: nat) (b: nat): constant :=
+  match op with
+  | op_plus =>  (cnat (a + b))
+  | op_eq =>  (cbool (Nat.eqb a b))
+  | op_lt =>  (cbool (Nat.ltb a b))
+  end.
+
+Notation "'[' x ':=' s ']' t" := (subst x s t) (at level 20).
+Notation "'[' x ':=' s ']v' t" := (value_subst x s t) (at level 20).
+
+Global Hint Constructors value: core.
+Global Hint Constructors tm: core.
+
+Reserved Notation "t1 '-->' t2" (at level 40).
+
+Inductive step : tm -> tm -> Prop :=
+| ST_Lete1: forall x e1 e1' e, e1 --> e1' -> (tlete x e1 e) --> (tlete x e1' e)
+| ST_Lete2: forall x v1 e, (tlete x (tvalue v1) e) --> (subst x v1 e)
+| ST_LetOp: forall x op n1 n2 e,
+    (tletbiop x op (vconst (cnat n1)) (vconst (cnat n2)) e) --> (subst x (vconst (apply_op op n1 n2)) e)
+| ST_LetAppLam: forall T x y v_x e1 e,
+    (tletapp y ((vlam x T e1)) v_x e) --> tlete y (subst x v_x e1) e
+where "t1 '-->' t2" := (step t1 t2).
+
+Notation multistep := (multi step).
+Notation "t1 '-->*' t2" := (multistep t1 t2) (at level 40).
+Notation step_normal_form := (normal_form step).
+
+Lemma value__normal : forall v, step_normal_form (tvalue v).
+Proof with eauto.
+  intro v. unfold normal_form.
+  induction v; intro HF; inversion HF; inversion H.
+Qed.
+
+Global Hint Constructors step: core.
+
+Definition op_ret_ty (op: biop): basic_ty :=
+  match op with
+  | op_plus => TNat
+  | op_eq => TBool
+  | op_lt => TBool
+  end.
