proof/DenotationSimp.v
@@ -1,0 +1,230 @@
+(** * MoreStlc: More on the Simply Typed Lambda-Calculus *)
+
+Set Warnings "-notation-overridden,-parsing".
+From PLF Require Import Maps.
+From PLF Require Import CoreLangSimp.
+From PLF Require Import NormalTypeSystemSimp.
+From PLF Require Import LinearContext.
+From PLF Require Import RfTypeDef.
+From PLF Require Import WellFormedSimp.
+From Coq Require Import Logic.FunctionalExtensionality.
+From Coq Require Import Logic.ClassicalFacts.
+From Coq Require Import Lists.List.
+
+Import CoreLangSimp.
+Import LinearContext.
+Import WellFormedSimp.
+Import ListNotations.
+
+Definition empstate: state := t_empty (cbool false).
+
+Definition context := linear_context overunderty.
+
+Definition empty_ctx: context := nil.
+
+Definition constant_basic_type_infer (c: constant) :=
+  match c with
+  | cbool _ => TBool
+  | cnat _ => TNat
+  end.
+
+Lemma constant_basic_type_infer_refl (c: constant) : forall (T:basic_ty), empty |- vconst c \Vin T <-> constant_basic_type_infer c = T.
+Proof with eauto.
+  induction c; split; intros; subst; eauto; try (inversion H; eauto).
+Qed.
+
+Global Hint Rewrite constant_basic_type_infer_refl: core.
+
+Lemma constant_basic_type_infer_spec (c: constant) : empty |- vconst c \Vin (constant_basic_type_infer c).
+Proof with eauto.
+  induction c...
+Qed.
+
+Global Hint Resolve constant_basic_type_infer_spec: core.
+
+Definition mk_eq_constant c := [[v: constant_basic_type_infer c | (fun _ v => v = c) ]].
+Definition mk_bot ty := [[v: ty | (fun _ _ => False) ]].
+Definition mk_top ty := [[v: ty | (fun _ _ => True) ]].
+Definition mk_eq_var ty name := [[v: ty | (fun state v => v = (state name)) ]].
+
+Lemma mk_eq_constant_spec (c: constant) : empty |- vconst c \in u\_ mk_eq_constant c _/.
+Proof with eauto.
+  induction c...
+Qed.
+
+Lemma subst_constant_eq: forall x c_x c, (<u[ x |c-> c_x ]> mk_eq_constant c) = mk_eq_constant c.
+Proof.
+  intros. simpl.
+  assert (<r[ x |c-> c_x ]> (fun (_ : state) (v : constant) => v = c) = (fun (_ : state) (v : constant) => v = c)).
+  unfold refinement_subst_c.
+  apply functional_extensionality. intros. apply functional_extensionality. auto.
+  setoid_rewrite H. auto.
+Qed.
+
+Lemma constant_eq_is_close: forall Gamma c, well_formed Gamma (mk_eq_constant c).
+Proof.
+  intros. constructor.
+  assert (well_formed_refinement nil (constant_basic_type_infer c) (fun (_ : state) (v : constant) => v = c)).
+  constructor.
+  unfold is_closed_refinement; destruct c; simpl; reflexivity.
+  apply well_formed_refinement_weakening with (Gamma1 := (erase_basetypectx (lcontxt_to_baseconctx Gamma))) (Gamma2 := nil); auto.
+  rewrite app_nil_r. auto.
+Qed.
+
+Global Hint Resolve mk_eq_constant_spec: core.
+Global Hint Resolve subst_constant_eq: core.
+Global Hint Resolve constant_eq_is_close: core.
+
+Definition phi_is_bot (phi: refinement):= forall st c, ~ phi st c.
+
+(* logical relation *)
+
+Definition is_constant (v: value) :=
+  match v with
+  | vconst _ => True
+  | _ => False
+  end.
+
+(* overtype denotation *)
+Definition over_tmR (ty:overbasety) (c:constant) : Prop :=
+  empty |- c \Vin o\_ ty _/ /\
+            (match ty with
+             | {{v: T | phi }} =>
+                 is_closed_refinement T phi /\ (phi empstate c)
+             end).
+
+Inductive is_application: tm -> value -> tm -> Prop :=
+| Is_application: forall (e1: tm) (v2: value) (f x: string),
+    ~ f \FVtm v2 -> is_application e1 v2 (tlete f e1 (tletapp x f v2 x)).
+
+(* Inductive under_tmR: underty -> tm -> Prop := *)
+(* | under_tmR_base: forall (T: basic_ty) phi e, *)
+(*     empty |- e \in T -> is_closed_refinement T phi -> *)
+(*                   (forall (c: constant), empty |- vconst c \Vin T -> *)
+(*                                             (phi empstate c -> e -->* (vconst c))) -> *)
+(*                   under_tmR ([[v: T | phi]]) e *)
+(* | under_tmR_oarr: forall x t1 t2 e, *)
+(*     empty |- e \in u\_ x o: t1 o--> t2 _/ -> *)
+(*                            (forall (c_x: constant), *)
+(*                                over_tmR t1 c_x -> *)
+(*                                (forall e3, is_application e c_x e3 -> under_tmR (under_subst_c x c_x t2) e3)) -> *)
+(*                            under_tmR (x o: t1 o--> t2) e *)
+(* | under_tmR_arrarr: forall t1 t2 e, *)
+(*     empty |- e \in u\_ t1 u--> t2 _/ -> *)
+(*                   ( forall (e_x: tm), *)
+(*                       under_tmR t1 e_x -> *)
+(*                       (forall (v_x: value), *)
+(*                           empty |- v_x \Vin u\_ t1 _/ -> *)
+(*                                   e -->* v_x -> *)
+(*                                   (forall e3, is_application e v_x e3 -> under_tmR t2 e3) *)
+(*                   )) -> *)
+(*                   under_tmR (t1 u--> t2) e. *)
+
+
+Fixpoint under_arr_tmR_aux (ty:underarrowty) (e:tm) : Prop :=
+  empty |- e \in u\_ ty _/ /\
+                  (match ty with
+                   | x o: t1 o--> t2 => False
+                   | t1 u--> t2 =>
+                       forall (e_x: tm),
+                         under_arr_tmR_aux t1 e_x ->
+                         (forall (v_x: value),
+                             empty |- v_x \Vin u\_ t1 _/ ->
+                                     e -->* v_x ->
+                                     (forall e3, is_application e v_x e3 -> under_tmR_aux t2 e3)
+                         )
+                   end)
+with under_tmR_aux (ty:underty) (e:tm) : Prop :=
+       empty |- e \in u\_ ty _/ /\
+                       (match ty with
+                        | [[v: T | phi ]] =>
+                            is_closed_refinement T phi /\
+                              (forall (c: constant),
+                                  empty |- vconst c \Vin T ->
+                                          (phi empstate c -> e -->* (vconst c))
+                              )
+                        | ArrowUnder ty => under_arr_tmR_aux ty e
+                        end).
+
+Definition under_tmR (ty:underty) (e:tm) : Prop :=
+  empty |- e \in u\_ ty _/ /\
+                  (match ty with
+                   | [[v: _ | _ ]] => under_tmR_aux ty e
+                   | _ u--> _ => under_tmR_aux ty e
+                   | x o: t1 o--> t2 =>
+                       forall (c_x: constant),
+                         over_tmR t1 c_x -> (forall e3, is_application e c_x e3 -> under_tmR_aux (under_subst_c x c_x t2) e3)
+                   end).
+
+Inductive tmR: overunderty -> tm -> Prop :=
+| tmR_oty: forall oty c, over_tmR oty c -> tmR oty c
+| tmR_uty: forall uty e, under_tmR uty e -> tmR uty e.
+
+Lemma tmR_constant (c: constant): tmR (mk_eq_constant c) (vconst c).
+Proof with eauto.
+  constructor. split; auto.
+  destruct c; simpl; split; auto; split; intros; subst...
+Qed.
+
+Global Hint Resolve tmR_constant: core.
+
+Fixpoint ty_subst_under_ctx (id:string) (c_id: constant) (Gamma: context) (tau: underty) : context * underty :=
+  match Gamma with
+  | nil => (Gamma, underty_subst id c_id tau)
+  | (x, xty) :: Gamma =>
+      if String.eqb x id
+      then
+        ((x, overunder_subst_c id c_id xty) :: Gamma, tau)
+      else
+        let (Gamma', tau') := (ty_subst_under_ctx id c_id Gamma tau) in
+        ((x, overunder_subst_c id c_id xty) :: Gamma', tau')
+  end.
+
+Lemma ty_subst_under_ctx_not_in_ctx (id:string) (c_id: constant) (Gamma: context) (tau: underty):
+  l_find_right_most Gamma id = None ->
+  ty_subst_under_ctx id c_id Gamma tau = (Gamma, (underty_subst id c_id tau)).
+Admitted.
+
+
+Inductive tmR_in_ctx: context -> underty -> tm -> Prop :=
+| tmR_in_ctx_nil: forall (ty: underty) e, tmR ty e -> tmR_in_ctx [] ty e
+| tmR_in_ctx_cons_over: forall (x: string) (T:basic_ty) (phi: refinement) (Gamma: context) tau e,
+    (forall c_x Gamma' tau', over_tmR ({{v: T | phi}}) c_x ->
+                        (Gamma', tau') = ty_subst_under_ctx x c_x Gamma tau ->
+                        tmR_in_ctx Gamma' tau' (subst x (vconst c_x) e)) ->
+    tmR_in_ctx ((x, (Oty ({{v: T | phi}}))) :: Gamma) tau e
+| tmR_in_ctx_cons_under: forall (x: string) (T:basic_ty) (phi: refinement) (Gamma: context) tau e,
+    (exists e_x, under_tmR ([[v: T | phi]]) e_x /\
+              (forall (c_x: constant) Gamma' tau',
+                  empty |- (vconst c_x) \Vin T -> e_x -->* (vconst c_x) ->
+                          (Gamma', tau') = ty_subst_under_ctx x c_x Gamma tau ->
+                          tmR_in_ctx Gamma' tau' (subst x (vconst c_x) e))) ->
+    tmR_in_ctx ((x, (Uty ([[v: T | phi]]))) :: Gamma) tau e
+| tmR_in_ctx_cons_ind_arrow: forall (x: string) t1 t2 (Gamma: context) (ty: underty) e,
+    (exists e_x, under_tmR (t1 u--> t2) e_x /\
+              tmR_in_ctx Gamma ty (tlete x e_x e)) ->
+    tmR_in_ctx ((x, Uty (t1 u--> t2)) :: Gamma) ty e
+| tmR_in_ctx_cons_d_arrow: forall (x: string) (y: string) (t1: overbasety) (t2: underty) (Gamma: context) (ty: underty) e,
+    (exists e_x, under_tmR (y o: t1 o--> t2) e_x /\
+              tmR_in_ctx Gamma ty (tlete x e_x e)) ->
+    tmR_in_ctx ((x, Uty (y o: t1 o--> t2)) :: Gamma) ty e.
+
+Global Hint Constructors tmR_in_ctx: core.
+
+Lemma tmR_in_ctx_pre_weakening: forall Gamma1 Gamma2 Gamma3 (tau: underty),
+    (Gamma1 ++ Gamma2) = Gamma3 ->
+    well_formed Gamma2 tau ->
+    (forall e, tmR_in_ctx Gamma2 tau e -> tmR_in_ctx Gamma3 tau e).
+Admitted.
+
+Definition context_not_free_in_term {A: Type} (ctx: linear_context A) (e: tm): Prop.
+Admitted.
+
+Definition context_not_free_in_underty {A: Type} (ctx: linear_context A) (tau: underty): Prop.
+Admitted.
+
+Lemma tmR_in_ctx_post_weakening: forall Gamma (tau: underty),
+    well_formed l_empty tau ->
+    (forall e, tmR_in_ctx l_empty tau e -> tmR_in_ctx Gamma tau e).
+Proof with eauto.
+Admitted.
