proof/NormalTypeSystemSimp.v
@@ -1,0 +1,285 @@
+Set Warnings "-notation-overridden,-parsing".
+From PLF Require Import Maps.
+From PLF Require Import Types.
+From PLF Require Import Smallstep.
+From PLF Require Import CoreLangSimp.
+
+Ltac invert :=
+  match goal with | H : ?T |- _ =>
+                      match type of T with Prop => solve [exfalso; apply H; auto]
+                      end
+  end.
+
+Import CoreLangSimp.
+
+Definition context := partial_map ty.
+
+Reserved Notation "Gamma '|-' t '\in' T" (at level 40).
+
+Inductive has_type : context -> tm -> ty -> Prop :=
+| T_Exn : forall Gamma T, has_type Gamma texn T
+| T_Value : forall Gamma value T,
+    value_has_type Gamma value T -> has_type Gamma (tvalue value) T
+| T_Lete : forall Gamma x e1 e2 T1 T2,
+    has_type Gamma e1 T1 ->
+    has_type (update Gamma x T1) e2 T2 ->
+    has_type Gamma (tlete x e1 e2) T2
+| T_LetOp : forall Gamma x op v1 v2 e2 T2,
+    value_has_type Gamma v1 (TBasic TNat) ->
+    value_has_type Gamma v2 (TBasic TNat) ->
+    has_type (update Gamma x (TBasic (op_ret_ty op))) e2 T2 ->
+    has_type Gamma (tletbiop x op v1 v2 e2) T2
+| T_LetApp : forall Gamma y v_x v_f e2 T_x T_y T2,
+    value_has_type Gamma v_x T_x ->
+    value_has_type Gamma v_f (TArrow T_x T_y) ->
+    has_type (update Gamma y T_y) e2 T2 ->
+    has_type Gamma (tletapp y v_f v_x e2) T2
+with value_has_type : context -> value -> ty -> Prop :=
+| T_ConstantB : forall Gamma b, value_has_type Gamma (vconst (cbool b)) (TBasic TBool)
+| T_ConstantI : forall Gamma n, value_has_type Gamma (vconst (cnat n)) (TBasic TNat)
+| T_Var : forall Gamma x T, Gamma x = Some T -> value_has_type Gamma (vvar x) T
+| T_Lam : forall Gamma x T11 T12 t12,
+    has_type (update Gamma x T11) t12 T12 ->
+    value_has_type Gamma (vlam x T11 t12) (TArrow T11 T12)
+
+where "Gamma '|-' t '\in' T" := (has_type Gamma t T).
+Notation "Gamma '|-' t '\Vin' T" := (value_has_type Gamma t T) (at level 40).
+
+Global Hint Constructors has_type: core.
+Global Hint Constructors value_has_type: core.
+
+Lemma op_type_safe: forall op n1 n2, empty |- vconst (apply_op op n1 n2) \Vin TBasic (op_ret_ty op).
+Proof.
+  intro op.
+  destruct op; simpl; intros; auto.
+Qed.
+
+Global Hint Resolve op_type_safe: core.
+
+Lemma nat_value_n_exists: forall v, empty |- v \Vin (TBasic TNat) -> (exists n, v = (vconst (cnat n))).
+Proof.
+  intros.
+  destruct v; inversion H; subst; eauto.
+  - inversion H2.
+Qed.
+
+Lemma bool_value_b_exists: forall v, empty |- v \Vin (TBasic TBool) -> (exists b, v = (vconst (cbool b))).
+Proof.
+  intros.
+  destruct v; inversion H; subst; eauto.
+  - inversion H2.
+Qed.
+
+Lemma basic_value_const_exists:
+  forall T v, empty |- v \Vin (TBasic T) -> (exists c, v = vconst c).
+Proof.
+  intros.
+  destruct v; inversion H; subst; eauto. inversion H2.
+Qed.
+
+Lemma arrow_value_lam_exists: forall v T1 T2,
+    empty |- v \Vin (TArrow T1 T2) -> exists x e, v = vlam x T1 e.
+Proof.
+  intros.
+  destruct v; inversion H; subst; eauto.
+  - inversion H2.
+Qed.
+
+Lemma has_type_inv_value: forall Gamma v T, Gamma |- tvalue v \in T -> Gamma |- v \Vin T.
+Proof.
+  intros.
+  inversion H; subst; auto.
+Qed.
+
+Definition halts (t:tm) : Prop :=  exists t', t -->* t' /\ is_value t' = true.
+
+Lemma value_halts : forall v, halts (tvalue v).
+Proof.
+  intros v. unfold halts. exists (tvalue v). split; auto.
+Qed.
+
+Lemma weakening : forall e T Gamma Gamma',
+    includedin Gamma Gamma' ->
+    (Gamma  |- e \in T -> Gamma' |- e \in T).
+Proof.
+  intro e.
+  apply (tm_mutual_rec
+         (fun v => forall T Gamma Gamma', includedin Gamma Gamma' -> (Gamma  |- v \Vin T -> Gamma' |- v \Vin T))
+         (fun e => forall T Gamma Gamma', includedin Gamma Gamma' -> (Gamma  |- e \in T -> Gamma' |- e \in T))).
+  - intros; inversion H0; subst; eauto 7 using includedin_update.
+  - intros; inversion H0; subst; eauto 7 using includedin_update.
+  - intros; inversion H1; subst; eauto 7 using includedin_update.
+  - intros; inversion H0; subst; eauto 7 using includedin_update.
+  - intros. inversion H1; subst; eauto 7 using includedin_update.
+  - intros; inversion H2; subst; eauto 7 using includedin_update.
+  - intros; inversion H3; subst; eauto 7 using includedin_update.
+  (* - intros. inversion H2; subst; eauto 7 using includedin_update. *)
+  - intros; inversion H3; subst; eauto 7 using includedin_update.
+Qed.
+
+Lemma value_weakening : forall e T Gamma Gamma',
+    includedin Gamma Gamma' ->
+    (Gamma  |- e \Vin T -> Gamma' |- e \Vin T).
+Proof.
+  intros.
+  apply weakening with (e:=tvalue e) (T:=T) in H; auto.
+  inversion H; subst; auto.
+Qed.
+
+Lemma weakening_empty : forall Gamma t T,
+    empty |- t \in T  -> Gamma |- t \in T.
+Proof.
+  intros Gamma t T.
+  eapply weakening.
+  discriminate.
+Qed.
+
+Lemma value_weakening_empty : forall Gamma t T,
+    empty |- t \Vin T  -> Gamma |- t \Vin T.
+Proof.
+  intros Gamma t T H.
+  assert (empty |- (tvalue t) \in T). auto.
+  apply weakening_empty with (Gamma:=Gamma) in H0. inversion H0; subst; auto.
+Qed.
+
+Lemma substitution_preserves_typing1:
+  (forall (c : constant) (Gamma : partial_map ty) (x : string) (U : ty) (v : value) (T : ty),
+      (x |-> U; Gamma) |- vconst c \Vin T -> empty |- v \Vin U -> Gamma |- [x := v ]v vconst c \Vin T).
+Proof.
+  intro c. induction c; intros; inversion H; clear H; subst; simpl; eauto.
+Qed.
+
+Lemma substitution_preserves_typing2:
+  (forall (s : string) (Gamma : partial_map ty) (x : string) (U : ty) (v : value) (T : ty),
+      (x |-> U; Gamma) |- s \Vin T -> empty |- v \Vin U -> Gamma |- [x := v ]v s \Vin T).
+Proof.
+  intros. inversion H; clear H; subst; simpl; eauto.
+  rename s into y. rename x into x.
+  destruct (eqb_spec x y); subst.
+  + (* x=y *)
+    rewrite update_eq in H3.
+    injection H3 as H3; subst.
+    apply value_weakening_empty. assumption.
+  + (* x<>y *)
+    apply T_Var. rewrite update_neq in H3; auto.
+Qed.
+
+Lemma substitution_preserves_typing5:
+  (forall v : value,
+      (forall (Gamma : partial_map ty) (x : string) (U : ty) (v0 : value) (T : ty),
+          (x |-> U; Gamma) |- v \Vin T -> empty |- v0 \Vin U -> Gamma |- [x := v0 ]v v \Vin T) ->
+      forall (Gamma : partial_map ty) (x : string) (U : ty) (v0 : value) (T : ty),
+        (x |-> U; Gamma) |- tvalue v \in T -> empty |- v0 \Vin U -> Gamma |- [x := v0] tvalue v \in T).
+Proof.
+  intros. inversion H0; clear H0; subst; simpl; eauto.
+Qed.
+
+Lemma substitution_preserves_typing7:
+  (forall (s : string) (t : tm),
+      (forall (Gamma : partial_map ty) (x : string) (U : ty) (v : value) (T : ty),
+          (x |-> U; Gamma) |- t \in T -> empty |- v \Vin U -> Gamma |- [x := v] t \in T) ->
+      forall t0 : tm,
+        (forall (Gamma : partial_map ty) (x : string) (U : ty) (v : value) (T : ty),
+            (x |-> U; Gamma) |- t0 \in T -> empty |- v \Vin U -> Gamma |- [x := v] t0 \in T) ->
+        forall (Gamma : partial_map ty) (x : string) (U : ty) (v : value) (T : ty),
+          (x |-> U; Gamma) |- tlete s t t0 \in T -> empty |- v \Vin U -> Gamma |- [x := v] tlete s t t0 \in T).
+Proof.
+  intros. inversion H1; clear H1; subst; simpl; eauto.
+  rename s into y. rename x into x.
+  destruct (eqb_spec x y); subst.
+  + (* x=y *)
+    rewrite update_shadow in H9.
+    apply T_Lete with (T1:= T1); auto. apply H with (U:=U); auto.
+  + (* x<>y *)
+    apply T_Lete with (T1:= T1); auto. apply H with (U:=U); auto.
+    rewrite update_permute in H9; auto. apply H0 with (U:=U); auto.
+Qed.
+
+Lemma substitution_preserves_typing8:
+  (forall (s : string) (b : biop) (v : value),
+      (forall (Gamma : partial_map ty) (x : string) (U : ty) (v0 : value) (T : ty),
+          (x |-> U; Gamma) |- v \Vin T -> empty |- v0 \Vin U -> Gamma |- [x := v0 ]v v \Vin T) ->
+      forall v0 : value,
+        (forall (Gamma : partial_map ty) (x : string) (U : ty) (v1 : value) (T : ty),
+            (x |-> U; Gamma) |- v0 \Vin T -> empty |- v1 \Vin U -> Gamma |- [x := v1 ]v v0 \Vin T) ->
+        forall t : tm,
+          (forall (Gamma : partial_map ty) (x : string) (U : ty) (v1 : value) (T : ty),
+              (x |-> U; Gamma) |- t \in T -> empty |- v1 \Vin U -> Gamma |- [x := v1] t \in T) ->
+          forall (Gamma : partial_map ty) (x : string) (U : ty) (v1 : value) (T : ty),
+            (x |-> U; Gamma) |- tletbiop s b v v0 t \in T ->  empty |- v1 \Vin U -> Gamma |- [x := v1] tletbiop s b v v0 t \in T).
+Proof.
+  intros. inversion H2; clear H2; subst; simpl; eauto.
+  rename s into y. rename x into x.
+  destruct (eqb_spec x y); subst.
+  + (* x=y *)
+    rewrite update_shadow in H13.
+    apply T_LetOp; auto. apply H with (U:=U); auto. apply H0 with (U:=U); auto.
+  + (* x<>y *)
+    apply T_LetOp; auto. apply H with (U:=U); auto.
+    rewrite update_permute in H13; auto. apply H0 with (U:=U); auto.
+    rewrite update_permute in H13; auto. apply H1 with (U:=U); auto.
+Qed.
+
+Lemma substitution_preserves_typing9:
+  (forall (s : string) (v : value),
+      (forall (Gamma : partial_map ty) (x : string) (U : ty) (v0 : value) (T : ty),
+          (x |-> U; Gamma) |- v \Vin T -> empty |- v0 \Vin U -> Gamma |- [x := v0 ]v v \Vin T) ->
+      forall v0 : value,
+        (forall (Gamma : partial_map ty) (x : string) (U : ty) (v1 : value) (T : ty),
+            (x |-> U; Gamma) |- v0 \Vin T -> empty |- v1 \Vin U -> Gamma |- [x := v1 ]v v0 \Vin T) ->
+        forall t : tm,
+          (forall (Gamma : partial_map ty) (x : string) (U : ty) (v1 : value) (T : ty),
+              (x |-> U; Gamma) |- t \in T -> empty |- v1 \Vin U -> Gamma |- [x := v1] t \in T) ->
+          forall (Gamma : partial_map ty) (x : string) (U : ty) (v1 : value) (T : ty),
+            (x |-> U; Gamma) |- tletapp s v v0 t \in T -> empty |- v1 \Vin U -> Gamma |- [x := v1] tletapp s v v0 t \in T).
+Proof.
+  intros. inversion H2; clear H2; subst; simpl; eauto.
+  rename s into y. rename x into x.
+  destruct (eqb_spec x y); subst.
+  + (* x=y *)
+    rewrite update_shadow in H12.
+    apply T_LetApp with (T_x:=T_x) (T_y:=T_y); auto. apply H0 with (U:=U); auto. apply H with (U:=U); auto.
+  + (* x<>y *)
+    rewrite update_permute in H12; auto.
+    apply T_LetApp with (T_x:=T_x) (T_y:=T_y); auto.
+    apply H0 with (U:=U); auto.
+    apply H with (U:=U); auto.
+    apply H1 with (U:=U); auto.
+Qed.
+
+Lemma substitution_preserves_typing : forall t Gamma x U v T,
+    (x |-> U ; Gamma) |- t \in T ->  empty |- v \Vin U  ->  Gamma |- [x:=v]t \in T.
+Proof with eauto.
+  intro t.
+  apply (tm_mutual_rec
+           (fun ev => forall Gamma x U v T, (x |-> U ; Gamma) |- ev \Vin T ->  empty |- v \Vin U ->  Gamma |- [x:=v]v ev \Vin T)
+           (fun e => forall Gamma x U v T, (x |-> U ; Gamma) |- e \in T ->  empty |- v \Vin U ->  Gamma |- [x:=v] e \in T)
+           substitution_preserves_typing1 substitution_preserves_typing2).
+  - intros. inversion H0; subst; simpl; eauto.
+    destruct (eqb_spec x s); subst.
+    + rewrite update_shadow in H7...
+    + rewrite update_permute in H7...
+  - intros. inversion H0; subst; simpl; eauto.
+  - intros. inversion H0; subst; simpl; eauto.
+  - apply substitution_preserves_typing7.
+  - apply substitution_preserves_typing8.
+  - apply substitution_preserves_typing9.
+Qed.
+
+Theorem preservation : forall t t' T,
+    empty |- t \in T  ->
+                  t --> t'  ->
+                  empty |- t' \in T.
+Proof with eauto.
+  intros t t' T HT. generalize dependent t'.
+  remember empty as Gamma.
+  induction HT;
+    intros t' HE; subst; inversion HE; subst...
+  - apply substitution_preserves_typing with T1...
+    inversion HT1; subst...
+  - apply substitution_preserves_typing with (TBasic (op_ret_ty op))...
+  (* - apply substitution_preserves_typing with TNat... *)
+  - apply T_Lete with (T1 := T_y)...
+    apply substitution_preserves_typing with T_x...
+    inversion H0; subst...
+Qed.
