proof/RfTypeDef.v
@@ -1,0 +1,93 @@
+Set Warnings "-notation-overridden,-parsing".
+From PLF Require Import Maps.
+From PLF Require Import Types.
+(* From PLF Require Import Smallstep. *)
+From PLF Require Import CoreLangSimp.
+
+Definition state := total_map constant.
+(* The second constant is the self reference; the refinement is untyped *)
+Definition refinement : Type := state -> constant -> Prop.
+Implicit Type HH : refinement.
+
+Definition refinment_subst (x:string) (c:constant) (phi:refinement) : refinement :=
+  fun st v => phi (t_update st x c) v.
+
+Inductive overbasety : Type :=
+| BaseOver: basic_ty -> refinement -> overbasety.
+
+Definition overbasety_subst (x:string) (c:constant) (oty:overbasety) : overbasety :=
+  match oty with
+  | BaseOver T phi => BaseOver T (refinment_subst x c phi)
+  end.
+
+Inductive underarrowty : Type :=
+| DependArrow : string -> overbasety -> underty -> underarrowty
+| IndependArrow : underarrowty -> underty -> underarrowty
+with underty: Type :=
+| BaseUnder: basic_ty -> refinement -> underty
+| ArrowUnder: underarrowty -> underty.
+
+Scheme underarrowty_mutual_rec := Induction for underarrowty Sort Type
+    with underty_mutual_rec := Induction for underty Sort Type.
+
+Fixpoint underarrowty_subst (id:string) (c:constant) (oty:underarrowty) : underarrowty :=
+  match oty with
+  | DependArrow x t1 t2 => DependArrow x (overbasety_subst id c t1)
+                                      (if String.eqb x id then t2 else underty_subst id c t2)
+  | IndependArrow t1 t2 => IndependArrow (underarrowty_subst id c t1) (underty_subst id c t2)
+  end
+with underty_subst (id:string) (c:constant) (oty:underty) : underty :=
+       match oty with
+       | BaseUnder T phi => BaseUnder T (refinment_subst id c phi)
+       | ArrowUnder ty => ArrowUnder (underarrowty_subst id c ty)
+       end.
+
+Inductive overunderty : Type :=
+| Uty: underty -> overunderty
+| Oty: overbasety -> overunderty.
+
+Definition overunderty_subst (id:string) (c:constant) (oty:overunderty) : overunderty :=
+  match oty with
+  | Uty ty => Uty (underty_subst id c ty)
+  | Oty ty => Oty (overbasety_subst id c ty)
+  end.
+
+Coercion ArrowUnder :underarrowty >-> underty.
+Coercion Uty : underty >-> overunderty.
+Coercion Oty : overbasety >-> overunderty.
+
+Definition over_to_under (ot: overbasety) :=
+  match ot with
+  | BaseOver t phi => BaseUnder t phi
+  end.
+
+Notation "'[[v:' t '|' r ']]'" := (BaseUnder t r) (at level 20).
+Notation "'{{v:' t '|' r '}}'" := (BaseOver t r) (at level 20).
+Notation " x 'o:' overbasety 'o-->' retty " := (DependArrow x overbasety retty) (at level 20).
+Notation " underty 'u-->' retty " := (IndependArrow underty retty) (at level 20).
+
+Fixpoint underarrowty_erase (ut: underarrowty) : ty :=
+  match ut with
+  | _ o: {{v: T1 | _ }} o--> retty => T1 t--> (underty_erase retty)
+  | t1 u--> t2 => (underarrowty_erase t1) t--> (underty_erase t2)
+  end
+with underty_erase (ut: underty) : ty :=
+       match ut with
+       | [[v: T | _ ]] => T
+       | ArrowUnder ut => underarrowty_erase ut
+       end.
+
+Definition overbasety_erase (aty: overbasety): ty :=
+  match aty with
+  | ({{v: T | _ }}) => T
+  end.
+
+Definition overunderty_erase (aty: overunderty): ty :=
+  match aty with
+  | Uty ty => underty_erase ty
+  | Oty ty => overbasety_erase ty
+  end.
+
+Notation " 'u\_' ty '_/' " := (underty_erase ty) (at level 30).
+Notation " 'o\_' ty '_/' " := (overbasety_erase ty) (at level 30).
+Notation " 'ou\_' ty '_/' " := (overunderty_erase ty) (at level 30).
