proof/Soundness.v
@@ -1,35 +1,145 @@
 Set Warnings "-notation-overridden,-parsing".
 From PLF Require Import Maps.
-From PLF Require Import Smallstep.
-From PLF Require Import CoreLang.
+From PLF Require Import CoreLangSimp.
+From PLF Require Import NormalTypeSystemSimp.
 From PLF Require Import LinearContext.
-From PLF Require Import NormalTypeSystem.
-From PLF Require Import RefinementType.
+From PLF Require Import RfTypeDef.
+From PLF Require Import WellFormedSimp.
+From PLF Require Import DenotationSimp.
+From PLF Require Import SubtypingSimp.
+From PLF Require Import TypingRules.
+From Coq Require Import Logic.FunctionalExtensionality.
+From Coq Require Import Logic.ClassicalFacts.
 From Coq Require Import Lists.List.
+
+Import CoreLangSimp.
+Import LinearContext.
+Import WellFormedSimp.
+Import DenotationSimp.
+Import SubtypingSimp.
+Import TypingRules.
 Import ListNotations.
 
-(* Import RefinementType. *)
-
-Lemma has_refinement_type_has_basic_type: forall (e: tm) (tau: uty),
-    empty \C- e \T--> tau -> (Maps.empty |- e \in (erase tau)).
-Admitted.
-
-Global Hint Resolve has_refinement_type_has_basic_type: core.
-
-Theorem soundness: forall (e: tm) (T: basic_ty) (phi: constant -> Prop),
-    empty \C- e \T--> [[v: T | closed_r phi ]] ->
-    forall c, T = constant_basic_type_infer c -> phi c -> e -->* (tvalue (vconst c)).
+(* constant *)
+Lemma mk_eq_constant_implies_emptyctx_denotation: forall (c : constant),
+    tmR_in_ctx l_empty (mk_eq_constant c) (vconst c).
 Proof with eauto.
-  intros e T phi H c HcT. subst.
-  assert (Maps.empty |- e \in (constant_basic_type_infer c )) as Hnt. apply has_refinement_type_has_basic_type in H...
-  induction H; intros.
-  - inversion Hnt; subst. destruct c; inversion H1. apply multi_R...
-  - admit.
-  - admit.
-  - admit.
-  - admit.
-  - admit.
-  - admit.
-  - admit.
+  intro c. destruct c...
+Qed.
+
+Lemma mk_eq_constant_implies_denotation: forall Gamma (c : constant),
+    tmR_in_ctx Gamma (mk_eq_constant c) (vconst c).
+Proof with eauto.
+  intros Gamma c.
+  apply tmR_in_ctx_pre_weakening with (Gamma1 := Gamma) (Gamma2 := l_empty); auto. rewrite app_nil_r...
+Qed.
+
+(* err *)
+Lemma err_typecheck_implies_err_denotation: forall Gamma,
+   forall (T : basic_ty), well_formed_ctx Gamma -> tmR_in_ctx Gamma (mk_bot T) texn.
+Proof with eauto.
+  intros.
+  assert (tmR_in_ctx l_empty (mk_bot T) texn). unfold mk_bot.
+  repeat constructor... intros. inversion H1.
+  apply tmR_in_ctx_pre_weakening with (Gamma1 := Gamma) (Gamma2 := l_empty)... rewrite app_nil_r...
+  constructor...
+Qed.
+
+Lemma under_base_representative: forall T phi, exists e,
+    under_tmR ([[v:T | phi]]) e /\ (forall (c: constant), e -->* c <-> (forall st, phi st = (fun c' => c = c'))).
+Admitted.
+
+(* under var *)
+Lemma under_var_implies_denotation: forall (Gamma: context),
+  forall (x : string) (tau : underty),
+    well_formed_ctx Gamma -> l_find_right_most Gamma x = Some (Uty tau) -> tmR_in_ctx Gamma tau x.
+Proof with eauto.
+  intros Gamma x tau Hwf Hfind. apply l_find_right_most_some_spec in Hfind.
+  destruct Hfind as (Gamma1 & Gamma2 & Hctxconcat & HGamma2). subst.
+  generalize dependent x. generalize dependent tau. generalize dependent Gamma2.
+  induction Gamma1; simpl; intros Gamma2 tau x Hwf Hfind.
+  - destruct tau.
+    + constructor.
+      destruct (under_base_representative b r) as (e_x & H1 & H2).
+      exists e_x. split... intros c_x Gamma' tau' H3 H4 H5. rewrite H2 in H4. simpl. rewrite eqb_refl.
+      rewrite ty_subst_under_ctx_not_in_ctx in H5...
+      assert (is_closed_refinement b r). eapply constant_refinement_is_closed. apply H4.
+      inversion H5; subst...
+      erewrite refinement_subst_c_closed_rf...
+      apply tmR_in_ctx_pre_weakening with (Gamma1 := Gamma2) (Gamma2 := l_empty)...
+      apply app_nil_r.
+      constructor. simpl. constructor...
+      constructor... constructor... constructor... constructor... split... intros. rewrite H4 in H6. subst...
+    + destruct u.
+      {
+        constructor. admit.
+      }
+      {
+        constructor. admit.
+      }
   - admit.
 Admitted.
+
+(* sub *)
+Lemma sub_implies_denotation: forall (Gamma: context),
+  forall (e : tm) (tau1 tau2 : underty),
+  l_empty \C- e \Tin tau1 ->
+  tmR_in_ctx l_empty tau1 e ->
+  l_empty \C- tau1 \<: tau2 -> well_formed l_empty tau2 -> well_formed_ctx Gamma -> tmR_in_ctx Gamma tau2 e.
+Proof with eauto.
+
+
+Lemma disj_typecheck_implies_disj_denotation: forall Gamma,
+  forall (e : tm) (tau1 tau2 tau3 : underty),
+  Gamma \C- e \Tin tau1 ->
+  tmR_in_ctx Gamma tau1 e ->
+  Gamma \C- e \Tin tau2 ->
+  tmR_in_ctx Gamma tau2 e -> Gamma \C- tau1 \tyor tau2 \tyeq tau3 -> well_formed l_empty tau3 -> tmR_in_ctx Gamma tau3 e.
+Proof with eauto.
+  unfold disjunct. intros. rewrite <- H3...
+Qed.
+
+Theorem soundness: forall (Gamma: context) (e: tm) (uty:underty),
+    Gamma \C- e \Tin uty -> tmR_in_ctx Gamma uty e.
+Proof with eauto.
+  apply (term_under_type_chek_rec
+           (fun Gamma v uty H => tmR_in_ctx Gamma uty (tvalue v))
+           (fun Gamma e uty H => tmR_in_ctx Gamma uty e)); intros Gamma.
+  (* constant *)
+  - intros. apply mk_eq_constant_implies_denotation.
+  (* var *) (* some context trick *)
+  - apply under_var_implies_denotation.
+  - admit.
+  (* lam *) (* some context trick *)
+  - admit. - admit.
+  (* value *)
+  - auto.
+  (* err *)
+  - apply err_typecheck_implies_err_denotation.
+  (* sub *) (* some context trick *)
+  - intros e tau1 tau2 Ht1 Hd1 Hsub Hwf2 Hwfctx. unfold 
+  (* merge *)
+  - unfold disjunct. intros. rewrite <- d...
+  (* lete *)
+  - admit.
+  (* letop *)
+  - admit.
+  (* letapp_funcarg *)
+  - admit.
+  (* letapp_const *)
+  - admit.
+  (* letapp_var *)
+  - admit.
+Admitted.
+
+Lemma coverage: forall (e: tm) (T:basic_ty) (phi: constant -> Prop),
+    l_empty \C- e \Tin [[v: T | fun _ c => phi c ]] ->
+    forall (c: constant), empty |- (vconst c) \Vin T -> phi c -> e -->* vconst c .
+Proof with eauto.
+  intros.
+  apply soundness in H.
+  inversion H; subst.
+  inversion H2; subst. simpl in H2, H4.
+  destruct H4 as (_ & _ & Hprop).
+  apply Hprop; auto.
+Qed
