proof/SubtypingSimp.v
@@ -1,0 +1,54 @@
+Set Warnings "-notation-overridden,-parsing".
+From PLF Require Import Maps.
+From PLF Require Import CoreLangSimp.
+From PLF Require Import NormalTypeSystemSimp.
+From PLF Require Import LinearContext.
+From PLF Require Import RfTypeDef.
+From PLF Require Import WellFormedSimp.
+From PLF Require Import DenotationSimp.
+From Coq Require Import Logic.FunctionalExtensionality.
+From Coq Require Import Logic.ClassicalFacts.
+From Coq Require Import Lists.List.
+
+Import CoreLangSimp.
+Import LinearContext.
+Import WellFormedSimp.
+Import DenotationSimp.
+Import ListNotations.
+
+Reserved Notation "Gamma '\C-' t1 '\<:' t2"  (at level 40).
+
+(* subtyping judgement *)
+Inductive is_subtype : context -> underty -> underty -> Prop :=
+| Sub_UBase: forall Gamma T phi1 phi2,
+    (forall e, under_tmR ([[v: T | phi1 ]]) e -> under_tmR ([[v: T | phi2 ]]) e) ->
+    Gamma \C- [[v: T | phi1 ]] \<: [[v: T | phi2 ]]
+| Sub_IndependArrow_IndependArrow: forall Gamma (tau11 tau21: underarrowty) (tau12 tau22: underty),
+    Gamma \C- tau21 \<: tau11 ->
+    Gamma \C- tau12 \<: tau22 ->
+    Gamma \C- tau11 u--> tau12 \<: tau21 u--> tau22
+| Sub_DependArrow_DependArrow: forall Gamma T x1 phi11 x2 phi21 (tau12 tau22: underty),
+    (* We flip the overty to underty here *)
+    Gamma \C- [[v: T | phi11 ]] \<: [[v: T | phi21 ]] ->
+    (Gamma <l> x2 :l: ({{v: T | phi21 }})) \C- (under_subst_id x1 x2 tau12) \<: tau22 ->
+    Gamma \C- x1 o: {{v: T | phi11 }} o--> tau12 \<: x2 o: {{v: T | phi21 }} o--> tau22
+
+where "Gamma '\C-' t1 '\<:' t2" := (is_subtype Gamma t1 t2).
+
+Lemma is_subtype_spec: forall Gamma t1 t2,
+    is_subtype Gamma t1 t2 ->
+    (forall e, tmR_in_ctx Gamma t1 e -> tmR_in_ctx Gamma t2 e).
+Admitted.
+
+(* closing judgement *)
+Definition closing_with_drop (Gamma1 Gamma2: context) (tau: underty) :=
+  well_formed Gamma1 tau /\ (forall e, tmR_in_ctx Gamma1 tau e <-> tmR_in_ctx (Gamma1 ++ Gamma2) tau e).
+
+Notation "Gamma1 '\<' Gamma2 '\>' '\C-' tau " := (closing_with_drop Gamma1 Gamma2 tau) (at level 40).
+
+(* disjunction judgement *)
+
+Definition disjunct (Gamma: context) (tau1 tau2 tau3: underty) :=
+  (forall e, tmR_in_ctx Gamma tau1 e /\ tmR_in_ctx Gamma tau2 e <-> tmR_in_ctx Gamma tau3 e).
+
+Notation "Gamma '\C-' tau1 '\tyor' tau2 '\tyeq' tau3 " := (disjunct Gamma tau1 tau2 tau3) (at level 40).
