proof/TypingRules.v
@@ -1,0 +1,120 @@
+Set Warnings "-notation-overridden,-parsing".
+From PLF Require Import Maps.
+From PLF Require Import CoreLangSimp.
+From PLF Require Import NormalTypeSystemSimp.
+From PLF Require Import LinearContext.
+From PLF Require Import RfTypeDef.
+From PLF Require Import WellFormedSimp.
+From PLF Require Import DenotationSimp.
+From PLF Require Import SubtypingSimp.
+From Coq Require Import Logic.FunctionalExtensionality.
+From Coq Require Import Logic.ClassicalFacts.
+From Coq Require Import Lists.List.
+
+Import CoreLangSimp.
+Import LinearContext.
+Import WellFormedSimp.
+Import DenotationSimp.
+Import SubtypingSimp.
+Import ListNotations.
+
+Definition apply_op_over_refinements op (phi1 phi2: refinement): refinement :=
+  (fun st v =>
+     forall n1 n2, phi1 st (cnat n1) -> phi2 st (cnat n2) ->
+              v = (apply_op op n1 n2)).
+
+Definition mk_op_retty op (phi1 phi2: refinement) :=
+  (BaseUnder (op_ret_ty op) (apply_op_over_refinements op phi1 phi2)).
+
+Definition const_order: constant -> constant -> Prop.
+Admitted.
+
+Lemma const_order_is_well_founded: well_founded const_order.
+Admitted.
+
+Reserved Notation "Gamma '\C-' t '\Tin' T" (at level 40).
+Reserved Notation "Gamma '\C-' t '\Vin' T" (at level 40).
+
+Inductive term_under_type_chek : context -> tm -> underty -> Prop :=
+| UT_Value: forall Gamma v uty,
+    well_formed_ctx Gamma ->
+    Gamma \C- v \Vin uty -> Gamma \C- (tvalue v) \Tin uty
+| UT_Exn: forall Gamma T,
+    well_formed_ctx Gamma ->
+    Gamma \C- texn \Tin (mk_bot T)
+| UT_Sub: forall Gamma e tau1 tau2,
+    l_empty \C- e \Tin tau1 ->
+    l_empty  \C- tau1 \<: tau2 ->
+    well_formed l_empty tau2 ->
+    well_formed_ctx Gamma ->
+    Gamma \C- e \Tin tau2
+| UT_Merge: forall Gamma e (tau1 tau2 tau3: underty),
+    Gamma \C- e \Tin tau1 ->
+    Gamma \C- e \Tin tau2 ->
+    (Gamma \C- tau1 \tyor tau2 \tyeq tau3) ->
+    well_formed l_empty tau3 ->
+    Gamma \C- e \Tin tau3
+| UT_Lete: forall (Gamma: context) x e_x tau_x tau_x' e tau,
+    Gamma \C- e_x \Tin tau_x ->
+    Gamma \C- tau_x \<: tau_x' ->
+    (Gamma <l> x :l: tau_x') \C- e \Tin tau ->
+    Gamma \< ((x, Uty tau_x')::nil) \> \C- tau ->
+    Gamma \C- (tlete x e_x e) \Tin tau
+| UT_LetOp: forall (Gamma: context) x op v1 v2 phi1 phi2 tau_x' e tau,
+    Gamma \C- v1 \Vin [[v: TNat | phi1 ]] ->
+    Gamma \C- v2 \Vin [[v: TNat | phi2 ]] ->
+    Gamma \C- (mk_op_retty op phi1 phi2) \<: tau_x' ->
+    (Gamma <l> x :l: tau_x') \C- e \Tin tau ->
+    Gamma \< ((x, Uty tau_x')::nil) \> \C- tau ->
+    Gamma \C- (tletbiop x op v1 v2 e) \Tin tau
+| UT_LetAppIndepend: forall Gamma x v1 v2 e tauarg tau_x tau_x' tau,
+    Gamma \C- v1 \Vin (tauarg u--> tau_x) ->
+    Gamma \C- v2 \Vin tauarg ->
+    Gamma \C- tau_x \<: tau_x' ->
+    (Gamma <l> x :l: tau_x') \C- e \Tin tau ->
+    Gamma \< ((x, Uty tau_x')::nil) \> \C- tau ->
+    Gamma \C- (tletapp x v1 v2 e) \Tin tau
+(* the value can only be constant or variables *)
+| UT_LetAppDepend1: forall Gamma x v1 (c2: constant) e T phi a tau_x tau_x' tau,
+    Gamma \C- v1 \Vin (a o: {{v: T | phi}} o--> tau_x) ->
+    Gamma \C- c2 \Vin [[v: T | phi]] ->
+    Gamma \C- (under_subst_c a c2 tau_x) \<: tau_x' ->
+    (Gamma <l> x :l: tau_x') \C- e \Tin tau ->
+    Gamma \< ((x, Uty tau_x')::nil) \> \C- tau ->
+    Gamma \C- (tletapp x v1 c2 e) \Tin tau
+| UT_LetAppDepend2: forall Gamma x v1 (x2: string) e T phi a tau_x tau_x' tau,
+    Gamma \C- v1 \Vin (a o: {{v: T | phi}} o--> tau_x) ->
+    Gamma \C- x2 \Vin [[v: T | phi]] ->
+    Gamma \C- (under_subst_id a x2 tau_x) \<: tau_x' ->
+    (Gamma <l> x :l: tau_x') \C- e \Tin tau ->
+    Gamma \< ((x, Uty tau_x')::nil) \> \C- tau ->
+    Gamma \C- (tletapp x v1 x2 e) \Tin tau
+with value_under_type_check : context -> value -> underty -> Prop :=
+| UT_Contant: forall Gamma c,
+    well_formed_ctx Gamma ->
+    Gamma \C- (vconst c) \Vin (mk_eq_constant c)
+| UT_VarUnder: forall Gamma x (tau: underty),
+    well_formed_ctx Gamma ->
+    l_find_right_most Gamma x = Some (Uty tau) ->
+    Gamma \C- (vvar x) \Vin tau
+| UT_VarOver: forall Gamma T x,
+    well_formed_ctx Gamma ->
+    (exists phi, l_find_right_most Gamma x = Some (Oty ({{v: T | phi}}))) ->
+    Gamma \C- (vvar x) \Vin (mk_eq_var T x)
+| UT_LamDep: forall Gamma x tau_x e tau,
+    well_formed Gamma (x o: tau_x o--> tau) ->
+    (Gamma <l> x :l: Oty tau_x) \C- e \Tin tau ->
+                                          Gamma \C- (vlam x (o\_ tau_x _/) e) \Vin (x o: tau_x o--> tau)
+| UT_LamIndep: forall Gamma x tau_x e tau,
+    well_formed Gamma (tau_x u--> tau) ->
+    (Gamma <l> x :l: Uty tau_x) \C- e \Tin tau ->
+                                          Gamma \C- (vlam x (u\_ tau_x _/) e) \Vin (tau_x u--> tau)
+where
+"Gamma '\C-' t '\Tin' T" := (term_under_type_chek Gamma t T) and "Gamma '\C-' t '\Vin' T" := (value_under_type_check Gamma t T).
+
+Scheme value_under_type_check_rec := Induction for value_under_type_check Sort Prop
+    with term_under_type_chek_rec := Induction for term_under_type_chek Sort Prop.
+
+Lemma type_judgement_implies_well_formed: forall Gamma e tau,
+    Gamma \C- e \Tin tau -> well_formed_ctx Gamma /\ well_formed Gamma tau.
+Admitted.
