proof/WellFormedSimp.v
@@ -1,0 +1,275 @@
+Set Warnings "-notation-overridden,-parsing".
+From PLF Require Import Maps.
+From PLF Require Import CoreLangSimp.
+From Coq Require Import Lists.List.
+From Coq Require Import Strings.String.
+From Coq Require Import Logic.FunctionalExtensionality.
+From Coq Require Import Logic.ClassicalFacts.
+From PLF Require Import NormalTypeSystemSimp.
+From PLF Require Import RfTypeDef.
+From PLF Require Import LinearContext.
+Import ListNotations.
+
+Definition is_closed_refinement (_: basic_ty) (phi: refinement): Prop := forall st st', phi st = phi st'.
+
+Global Hint Unfold is_closed_refinement: core.
+
+Lemma constant_refinement_is_closed: forall (c: constant) (phi: refinement),
+    (forall st : state, phi st = (fun c' => c = c')) -> (forall T, is_closed_refinement T phi).
+Proof.
+  intros.
+  intros st st'. rewrite H. rewrite H. auto.
+Qed.
+
+Example true_refinement: is_closed_refinement TNat (fun _ c => c = 3).
+Proof.
+  unfold is_closed_refinement. reflexivity.
+Qed.
+
+Definition ncontxt := linear_context ty.
+Definition lcontxt := linear_context overunderty.
+
+Inductive well_formed_refinement : ncontxt -> basic_ty -> refinement -> Prop :=
+| well_formed_refinement_nil: forall T phi, is_closed_refinement T phi -> well_formed_refinement [] T phi
+| well_formed_refinement_cons: forall x T Gamma Tphi phi,
+    (forall (c_x: constant), empty |- c_x \Vin T ->
+                                well_formed_refinement Gamma Tphi (fun st c => phi (t_update st x c_x) c)) ->
+    well_formed_refinement ((x, T) :: Gamma) Tphi phi.
+
+Global Hint Constructors well_formed_refinement: core.
+
+Lemma well_formed_refinement_weakening: forall Gamma1 Gamma2 Gamma3 T phi,
+    (Gamma1 ++ Gamma2) = Gamma3 ->
+    well_formed_refinement Gamma2 T phi ->
+    well_formed_refinement Gamma3 T phi.
+Admitted.
+
+Module ExCloseRefinement.
+
+(* When the type dismatch, it is equal to bottom refinement *)
+Example true_refinement2: is_closed_refinement TNat (fun _ c => c = true).
+Proof.
+  unfold is_closed_refinement. reflexivity.
+Qed.
+
+Example refinement_under_nctx: well_formed_refinement [("x"%string, TBasic TNat)] TNat (fun st c => c = st "x"%string).
+Proof.
+  constructor. intros.
+  apply nat_value_n_exists in H. destruct H; subst.
+  constructor. constructor; subst; auto.
+Qed.
+
+End ExCloseRefinement.
+
+Inductive overunderbasety : Type :=
+| Obase: basic_ty -> refinement -> overunderbasety
+| Ubase: basic_ty -> refinement -> overunderbasety.
+
+Definition basecontxt := linear_context overunderbasety.
+
+Fixpoint erase_basetypectx (Gamma: basecontxt): ncontxt :=
+  match Gamma with
+  | nil => nil
+  | (x, Obase T _)::Gamma => (x, TBasic T)::(erase_basetypectx Gamma)
+  | (x, Ubase T _)::Gamma => (x, TBasic T)::(erase_basetypectx Gamma)
+  end.
+
+Inductive well_formed_in_basectx : basecontxt -> overunderty -> Prop :=
+| well_formed_base1: forall Gamma (T: basic_ty) phi,
+    well_formed_refinement (erase_basetypectx Gamma) T phi ->
+    well_formed_in_basectx Gamma ({{v: T | phi}})
+| well_formed_base2: forall Gamma (T: basic_ty) phi,
+    well_formed_refinement (erase_basetypectx Gamma) T phi ->
+    well_formed_in_basectx Gamma ([[v: T | phi]])
+| well_formed_oarr: forall Gamma x T phi (tau: underty),
+    well_formed_in_basectx Gamma ({{v: T | phi}}) ->
+    well_formed_in_basectx ((x, Obase T phi) :: Gamma) tau ->
+    well_formed_in_basectx Gamma (x o: ({{v: T | phi}}) o--> tau)
+| well_formed_arrarr: forall Gamma (tau_x: underarrowty) (tau: underty),
+    well_formed_in_basectx Gamma tau_x ->
+    well_formed_in_basectx Gamma tau ->
+    well_formed_in_basectx Gamma (tau_x u--> tau).
+
+Global Hint Constructors well_formed_in_basectx: core.
+
+(* before erase refinement from the context, we will erase all function type bindings *)
+Fixpoint lcontxt_to_baseconctx (Gamma: lcontxt): basecontxt :=
+  match Gamma with
+  | nil => nil
+  | (x, ty)::Gamma =>
+      match ty with
+      | Oty ({{v: T | phi }}) => (x, Obase T phi)::(lcontxt_to_baseconctx Gamma)
+      | Uty ([[v: T | phi ]]) => (x, Ubase T phi)::(lcontxt_to_baseconctx Gamma)
+      | _ => (lcontxt_to_baseconctx Gamma)
+      end
+  end.
+
+Definition well_formed (Gamma: lcontxt) (tau: overunderty):=
+  well_formed_in_basectx (lcontxt_to_baseconctx Gamma) tau.
+
+Fixpoint erase_arr_bindings (Gamma: lcontxt): lcontxt :=
+  match Gamma with
+  | nil => nil
+  | (x, ty)::Gamma =>
+      match ty with
+      | Oty _ | Uty ([[v: _ | _ ]]) => (x, ty)::(erase_arr_bindings Gamma)
+      | _ => (erase_arr_bindings Gamma)
+      end
+  end.
+
+Lemma erase_arr_bindings_spec: forall (Gamma: lcontxt),
+    lcontxt_to_baseconctx Gamma = lcontxt_to_baseconctx (erase_arr_bindings Gamma).
+Proof.
+  intro Gamma. induction Gamma; auto.
+  destruct a as (x, xty).
+  destruct xty. destruct u; simpl; auto.
+  - rewrite IHGamma. auto.
+  - destruct o. simpl. rewrite IHGamma. auto.
+Qed.
+
+Lemma well_fromed_even_without_arr_bindings: forall Gamma tau,
+    well_formed Gamma tau <-> well_formed (erase_arr_bindings Gamma) tau.
+Proof.
+  unfold well_formed. setoid_rewrite <- erase_arr_bindings_spec. reflexivity.
+Qed.
+
+Inductive well_formed_ctx: lcontxt -> Prop :=
+| well_formed_ctx_nil: well_formed_ctx nil
+| well_fromed_ctx_cons: forall x tau_x Gamma,
+    well_formed_ctx Gamma ->
+    well_formed Gamma tau_x ->
+    well_formed_ctx (Gamma <l> x :l: tau_x).
+
+Global Hint Constructors well_formed_ctx: core.
+
+Lemma well_formed_ctx_prefix: forall Gamma1 Gamm2,
+    well_formed_ctx (Gamma1 ++ Gamm2) -> well_formed_ctx Gamma1.
+Admitted.
+
+Lemma well_fromed_ctx_even_without_arr_bindings: forall Gamma,
+    well_formed_ctx Gamma -> well_formed_ctx (erase_arr_bindings Gamma).
+Admitted.
+
+Definition appear_free_in_refinement (name: string) T (phi: refinement): Prop :=
+  (exists st (c1 c2:constant),
+      empty |- c1 \Vin T /\ empty |- c2 \Vin T /\
+      phi (t_update st name c1) <> phi (t_update st name c2)
+  ).
+
+Definition appear_free_in_overbasety (name: string) T (oty: overbasety): Prop :=
+  match oty with
+  | {{v: _ | phi }} => appear_free_in_refinement name T phi
+  end.
+
+Fixpoint appear_free_in_underarrowty (name: string) T (uty: underarrowty): Prop :=
+  match uty with
+  | DependArrow x xty retty =>
+      appear_free_in_overbasety name T xty \/ (x <> name /\ appear_free_in_underty name T retty)
+  | IndependArrow t1 t2 =>
+      appear_free_in_underarrowty name T t1 \/ appear_free_in_underty name T t2
+  end
+with appear_free_in_underty (name: string) T (uty: underty): Prop :=
+       match uty with
+       | [[v: _ | phi ]] => appear_free_in_refinement name T phi
+       | ArrowUnder ty => appear_free_in_underarrowty name T ty
+       end.
+
+Definition appear_free_in_overunderty (name: string) T (overunderty: overunderty): Prop :=
+  match overunderty with
+  | Uty uty => appear_free_in_underty name T uty
+  | Oty oty => appear_free_in_overbasety name T oty
+  end.
+Notation " x '\FVty' e " := (appear_free_in_overunderty x e) (at level 40).
+
+Fixpoint appear_free_in_tvalue (id:string) (v:value) : Prop :=
+  match v with
+  | vconst _ => False
+  | vvar x => x = id
+  | vlam x xty e => x <> id /\ appear_free_in_ttm id e
+  end
+with appear_free_in_ttm (id:string) (e:tm) : Prop :=
+       match e with
+       | tvalue v => appear_free_in_tvalue id v
+       | tlete x e_x e => appear_free_in_ttm id e_x \/ (x <> id /\ appear_free_in_ttm id e)
+       | tletbiop x op v1 v2 e =>
+           appear_free_in_tvalue id v1 \/ appear_free_in_tvalue id v2 \/ (x <> id /\ appear_free_in_ttm id e)
+       | tletapp x v1 v2 e =>
+           appear_free_in_tvalue id v1 \/ appear_free_in_tvalue id v2 \/ (x <> id /\ appear_free_in_ttm id e)
+       | vexn => False
+       end.
+
+Notation " x '\FVtm' e " := (appear_free_in_ttm x e) (at level 40).
+Notation " x '\FVvalue' e " := (appear_free_in_tvalue x e) (at level 40).
+
+Definition refinement_subst_id (x1 x2: string) (phi: refinement): refinement :=
+  (fun st c => phi (t_update st x1 (st x2)) c).
+
+Definition over_subst_id (x1 x2: string) (oty: overbasety): overbasety :=
+  match oty with
+    | BaseOver T phi => BaseOver T (refinement_subst_id x1 x2 phi)
+  end.
+
+Fixpoint under_arr_subst_id (x1 x2: string) (uty: underarrowty): underarrowty :=
+  match uty with
+  | DependArrow x xty retty =>
+      if String.eqb x1 x then
+        DependArrow x (over_subst_id x1 x2 xty) retty
+      else
+        DependArrow x (over_subst_id x1 x2 xty) (under_subst_id x1 x2 retty)
+  | IndependArrow t1 t2 =>
+      IndependArrow (under_arr_subst_id x1 x2 t1) (under_subst_id x1 x2 t2)
+  end
+with under_subst_id (x1 x2: string) (uty: underty): underty :=
+       match uty with
+       | BaseUnder T phi => BaseUnder T (refinement_subst_id x1 x2 phi)
+       | ArrowUnder ty => under_arr_subst_id x1 x2 ty
+       end.
+
+Notation " '<r[' x '|x->' y ']>' uty " := (refinement_subst_id x y uty) (at level 40).
+Notation " '<u[' x '|x->' y ']>' uty " := (under_subst_id x y uty) (at level 40).
+Notation " '<o[' x '|x->' y ']>' uty " := (over_subst_id x y uty) (at level 40).
+
+Definition refinement_subst_c (x1: string) (c2: constant) (phi: refinement): refinement :=
+  (fun st c => phi (t_update st x1 c2) c).
+
+Lemma refinement_subst_c_closed_rf: forall x1 c2 T phi,
+    is_closed_refinement T phi -> refinement_subst_c x1 c2 phi = phi.
+Proof.
+  intros.
+  unfold is_closed_refinement in H. unfold refinement_subst_c.
+  apply functional_extensionality. intros st.
+  rewrite H with (st' := (x1 !-> c2; st)).
+  auto.
+Qed.
+
+Definition over_subst_c (x1: string) (c2: constant) (oty: overbasety): overbasety :=
+  match oty with
+    | BaseOver T phi => BaseOver T (refinement_subst_c x1 c2 phi)
+  end.
+
+Fixpoint under_arr_subst_c (x1: string) (c2: constant) (uty: underarrowty): underarrowty :=
+  match uty with
+  | DependArrow x xty retty =>
+      if String.eqb x1 x then
+        DependArrow x (over_subst_c x1 c2 xty) retty
+      else
+        DependArrow x (over_subst_c x1 c2 xty) (under_subst_c x1 c2 retty)
+  | IndependArrow t1 t2 =>
+      IndependArrow (under_arr_subst_c x1 c2 t1) (under_subst_c x1 c2 t2)
+  end
+with under_subst_c (x1: string) (c2: constant) (uty: underty): underty :=
+       match uty with
+       | BaseUnder T phi => BaseUnder T (refinement_subst_c x1 c2 phi)
+       | ArrowUnder ty => under_arr_subst_c x1 c2 ty
+       end.
+
+Definition overunder_subst_c (x1: string) (c2: constant) (outy: overunderty): overunderty :=
+  match outy with
+  | Uty uty => under_subst_c x1 c2 uty
+  | Oty oty => over_subst_c x1 c2 oty
+  end.
+
+Notation " '<r[' x '|c->' y ']>' uty " := (refinement_subst_c x y uty) (at level 40).
+Notation " '<u[' x '|c->' y ']>' uty " := (under_subst_c x y uty) (at level 40).
+Notation " '<o[' x '|c->' y ']>' uty " := (over_subst_c x y uty) (at level 40).
+Notation " '<ou[' x '|c->' y ']>' uty " := (overunder_subst_c x y uty) (at level 40).
